Misc clean up.
- Put code and proofs of examples in a single file.
- Rename encode/decode to avoid conflicts with encode/decode (of the countable class) in stdpp.
- Remove useless imports.

theories/proto/branching.v
@@ -1,57 +1,52 @@
-From iris.proofmode Require Import tactics.
-From iris.program_logic Require Export weakestpre.
 From iris.heap_lang Require Import proofmode notation.
-From iris.algebra Require Import list auth excl.
-From iris.base_logic Require Import invariants.
 From osiris.proto Require Export proto_enc.
 
-Section DualBranch.
-  Context `{PROP : bi}.
-
-  Definition TSB (a : action)
-             (prot1 prot2 : proto val PROP) : proto val PROP :=
-    TSR' a (λ _, True)%I (λ v, if v : bool then prot1 else prot2).
-
-  Global Instance is_dual_tsb a1 a2 proto1 proto1' proto2 proto2' :
-    IsDualAction a1 a2 →
-    IsDualProto proto1 proto1' → IsDualProto proto2 proto2' →
-    IsDualProto (TSB a1 proto1 proto2) (TSB a2 proto1' proto2').
-  Proof.
-    rewrite /IsDualAction.
-    rewrite /IsDualProto.
-    intros Ha Hst1 Hst2.
-    destruct a1.
-    - simpl.
-      simpl in Ha. rewrite -Ha.
-      rewrite -(proto_force_eq (dual_proto _)).
-      constructor.
-      f_equiv.
-      f_equiv.
-      destruct (decode a).
-      by destruct b. apply is_dual_end.
-    - simpl.
-      simpl in Ha. rewrite -Ha.
-      rewrite -(proto_force_eq (dual_proto _)).
-      constructor.
-      f_equiv.
-      f_equiv.
-      destruct (decode a).
-      by destruct b.
-      apply is_dual_end.
-  Qed.
-End DualBranch.
+Definition TSB {PROP : bi} (a : action)
+    (prot1 prot2 : proto val PROP) : proto val PROP :=
+  TSR' a (λ _, True)%I (λ v, if v : bool then prot1 else prot2).
 Global Typeclasses Opaque TSB.
-
 Infix "<+>" := (TSB Send) (at level 85) : proto_scope.
 Infix "<&>" := (TSB Receive) (at level 85) : proto_scope.
 
-Section branching_specs.
-  Context `{!heapG Σ} (N : namespace).
-  Context `{!logrelG val Σ}.
+Definition select : val := λ: "c" "s" "b", send "c" "s" "b".
+Definition branch : val := λ: "c" "s" "b1" "b2",
+  if: recv "c" "s" then "b1" else "b2".
+(* TODO: This notation should be fixed *)
+Notation "'branch:' c @ s 'left' e1 'right' e2" :=
+  (branch c s (λ: <>, e1)%E (λ: <>, e2)%E #())
+    (at level 200, c, s, e1, e2 at level 200) : expr_scope.
 
-  Definition select : val :=
-    λ: "c" "s" "b",
-      send "c" "s" "b".
+Global Instance is_dual_tsb {PROP : bi} a1 a2
+    (proto1 proto1' proto2 proto2' : proto val PROP) :
+  IsDualAction a1 a2 →
+  IsDualProto proto1 proto1' → IsDualProto proto2 proto2' →
+  IsDualProto (TSB a1 proto1 proto2) (TSB a2 proto1' proto2').
+Proof.
+  rewrite /IsDualAction.
+  rewrite /IsDualProto.
+  intros Ha Hst1 Hst2.
+  destruct a1.
+  - simpl.
+    simpl in Ha. rewrite -Ha.
+    rewrite -(proto_force_eq (dual_proto _)).
+    constructor.
+    f_equiv.
+    f_equiv.
+    destruct (val_decode a).
+    by destruct b. apply is_dual_end.
+  - simpl.
+    simpl in Ha. rewrite -Ha.
+    rewrite -(proto_force_eq (dual_proto _)).
+    constructor.
+    f_equiv.
+    f_equiv.
+    destruct (val_decode a).
+    by destruct b.
+    apply is_dual_end.
+Qed.
+
+Section branching_specs.
+  Context `{!heapG Σ, !logrelG val Σ} (N : namespace).
 
   Lemma select_st_spec proto1 proto2 γ c s (b : side) :
     {{{ ⟦ c @ s : proto1 <+> proto2 ⟧{N,γ} }}}
@@ -61,17 +56,9 @@ Section branching_specs.
     iIntros (Φ) "Hproto HΦ".
     wp_pures. wp_lam.
     wp_pures. rewrite /TSB.
-    wp_apply (send_st_spec N bool with "[$Hproto //]");
-    iIntros "Hstl".
-    iApply "HΦ".
-    by destruct b.
+    wp_apply (send_st_spec (A:=bool) with "[$Hproto //]"); iIntros "Hstl".
+    iApply "HΦ". by destruct b.
   Qed.
-  
-  Definition branch : val :=
-    λ: "c" "s" "b1" "b2",
-      if: recv "c" "s"
-       then "b1"
-       else "b2".
 
   Lemma branch_st_spec proto1 proto2 γ c s (b1 b2 : val) :
     {{{ ⟦ c @ s : proto1 <&> proto2 ⟧{N,γ} }}}
@@ -83,15 +70,9 @@ Section branching_specs.
     iIntros "Hproto HΦ'".
     wp_pures.
     wp_lam. rewrite /TSB. simpl.
-    wp_apply (recv_st_spec N bool with "[$Hproto //]").
-    iIntros (v) "[Hstl _]".
-    destruct v.
+    wp_apply (recv_st_spec (A:=bool) with "[$Hproto //]").
+    iIntros ([]) "[Hstl _]".
     - wp_pures. iApply ("HΦ'"). eauto with iFrame.
     - wp_pures. iApply ("HΦ'"). eauto with iFrame.
   Qed.
-
 End branching_specs.
-
-Notation "'branch:' c @ s 'left' e1 'right' e2" :=
-  (branch c s (λ: <>, e1)%E (λ: <>, e2)%E #())
-    (at level 200, c, s, e1, e2 at level 200) : expr_scope.
