theories/proto/encodable.v
@@ -1,151 +1,87 @@
-From iris.heap_lang Require Import proofmode notation.
+From iris.heap_lang Require Export notation.
 
-Class Encodable A := encode : A -> val.
-Class Decodable A := decode : val -> option A.
-Class EncDec (A : Type) {EA : Encodable A} {DA : Decodable A} :=
-{
-  encdec : ∀ v, decode (encode v) = Some v;
-  decenc : ∀ (v : val) (w : A) , decode v = Some w -> encode w = v
+Class ValEnc A := val_encode : A → val.
+Class ValDec A := val_decode : val → option A.
+Class ValEncDec A `{!ValEnc A, !ValDec A} := {
+  val_encode_decode v : val_decode (val_encode v) = Some v;
+  val_decode_encode v x : val_decode v = Some x → val_encode x = v;
 }.
 
-Ltac solve_encdec := intros v; by unfold decode, encode.
-Ltac solve_decenc :=
-  intros ?v ?w ?H;
-  destruct v as [?l | | | | ]; try by inversion H;
-  destruct l; try by inversion H.
-Ltac solve_encdec_decenc :=
-  split; [solve_encdec | solve_decenc].
+Local Arguments val_encode _ _ !_ /.
+Local Arguments val_decode _ _ !_ /.
+
+Lemma val_encode_decode_iff `{ValEncDec A} v x :
+  val_encode x = v ↔ val_decode v = Some x.
+Proof.
+  split; last apply val_decode_encode. intros <-. by rewrite -val_encode_decode.
+Qed.
+Instance val_encode_inj `{ValEncDec A} : Inj (=) (=) val_encode.
+Proof.
+  intros x y Heq. apply (inj Some).
+  by rewrite -(val_encode_decode x) Heq val_encode_decode.
+Qed.
 
 (* Instances *)
-Instance val_encodable : Encodable val := id.
-Instance val_decodable : Decodable val := id $ Some.
-Instance val_encdec : EncDec val.
+Instance val_val_enc : ValEnc val := id.
+Instance val_val_dec : ValDec val := id $ Some.
+Instance val_val_enc_dec : ValEncDec val.
+Proof. split. done. by intros ?? [= ->]. Qed.
+
+Instance int_val_enc : ValEnc Z := λ n, #n.
+Instance int_val_dec : ValDec Z := λ v,
+  match v with LitV (LitInt z) => Some z | _ => None end.
+Instance int_val_enc_dec : ValEncDec Z.
+Proof. split. done. by intros [[]| | | |] ? [= ->]. Qed.
+
+Instance bool_val_enc : ValEnc bool := λ b, #b.
+Instance bool_val_dec : ValDec bool := λ v,
+  match v with LitV (LitBool b) => Some b | _ => None end.
+Instance bool_val_enc_dec : ValEncDec bool.
+Proof. split. done. by intros [[]| | | |] ? [= ->]. Qed.
+
+Instance loc_val_enc : ValEnc loc := λ l, #l.
+Instance loc_val_dec : ValDec loc := λ v,
+  match v with LitV (LitLoc l) => Some l | _ => None end.
+Instance loc_val_enc_dec : ValEncDec loc.
+Proof. split. done. by intros [[]| | | |] ? [= ->]. Qed.
+
+Instance unit_val_enc : ValEnc unit := λ _, #().
+Instance unit_val_dec : ValDec unit := λ v,
+  match v with LitV LitUnit => Some () | _ => None end.
+Instance unit_val_enc_dec : ValEncDec unit.
+Proof. split. by intros []. by intros [[]| | | |] ? [= <-]. Qed.
+
+Instance pair_val_enc `{ValEnc A, ValEnc B} : ValEnc (A * B) := λ p,
+  (val_encode p.1, val_encode p.2)%V.
+Instance pair_val_dec `{ValDec A, ValDec B} : ValDec (A * B) := λ v,
+  match v with
+  | PairV v1 v2 => x1 ← val_decode v1; x2 ← val_decode v2; Some (x1, x2)
+  | _ => None
+  end.
+Instance pair_val_enc_dec `{ValEncDec A, ValEncDec B} : ValEncDec (A * B).
 Proof.
   split.
-  - intros v. unfold decode, encode. eauto.
-  - intros v w H. by destruct v; inversion H.
+  - intros []. by rewrite /= val_encode_decode /= val_encode_decode.
+  - intros [] ??; simplify_option_eq;
+      by repeat match goal with
+      | H : val_decode _ = Some _ |- _ => apply val_decode_encode in H as <-
+      end.
 Qed.
 
-Instance int_encodable : Encodable Z := λ n, #n.
-Instance int_decodable : Decodable Z :=
-  λ v, match v with
-       | LitV (LitInt z) => Some z
-       | _ => None
-       end.
-Instance int_encdec : EncDec Z.
-Proof. solve_encdec_decenc. Qed.
-
-Instance bool_encodable : Encodable bool := λ b, #b.
-Instance bool_decodable : Decodable bool :=
-  λ v, match v with
-       | LitV (LitBool b) => Some b
-       | _ => None
-       end.
-Instance bool_encdec : EncDec bool.
-Proof. solve_encdec_decenc. Qed.
-
-Instance loc_encodable : Encodable loc := λ l, #l.
-Instance loc_decodable : Decodable loc :=
-  λ v, match v with
-       | LitV (LitLoc l) => Some l
-       | _ => None
-       end.
-Instance loc_encdec : EncDec loc.
-Proof. solve_encdec_decenc. Qed.
-
-Instance unit_encodable : Encodable unit := λ _, #().
-Instance unit_decodable : Decodable unit :=
-  λ v, match v with
-       | LitV (LitUnit) => Some ()
-       | _ => None
-       end.
-Instance unit_encdec : EncDec unit.
+Instance option_val_enc `{ValEnc A} : ValEnc (option A) := λ mx,
+  match mx with Some x => SOMEV (val_encode x) | None => NONEV end%V.
+Instance option_val_dec `{ValDec A} : ValDec (option A) := λ v,
+  match v with
+  | SOMEV v => x ← val_decode v; Some (Some x)
+  | NONEV => Some None
+  | _ => None
+  end.
+Instance option_val_enc_dec `{ValEncDec A} : ValEncDec (option A).
 Proof.
   split.
-  - intros v. destruct v. by unfold decode, encode.
-  - solve_decenc.
-Qed.
-
-Instance pair_encodable `{Encodable A, Encodable B} : Encodable (A * B) :=
-  λ p, (encode p.1, encode p.2)%V.
-Instance pair_decodable `{Decodable A, Decodable B} : Decodable (A * B) :=
-  λ v, match v with
-       | PairV v1 v2 => match decode v1, decode v2 with
-                        | Some v1, Some v2 => Some (v1, v2)
-                        | _, _ => None
-                        end
-       | _ => None
-       end.
-Instance pair_encdec `{EncDec A, EncDec B} : EncDec (A * B).
-Proof.
-  split.
-  - intros v. destruct v. unfold decode, encode. simpl.
-    rewrite encdec. rewrite encdec. reflexivity.
-  - intros v w Heq. destruct w.
-    unfold decode, encode in *.
-    unfold pair_encodable, pair_decodable in *. simpl.
-    destruct v; inversion Heq.
-    by f_equiv;
-    apply decenc;
-    destruct (decode v1); inversion Heq;
-    destruct (decode v2); inversion Heq.
-Qed.
-
-Instance option_encodable `{Encodable A} : Encodable (option A) := λ mx,
-  match mx with Some x => SOMEV (encode x) | None => NONEV end%V.
-Instance option_decodable `{Decodable A} : Decodable (option A) :=
-  λ v, match v with
-       | SOMEV v => match decode v with
-                    | Some v => Some (Some v)
-                    | None => None
-                    end
-       | NONEV => Some (None)
-       | _ => None
-       end.
-Instance option_encdec `{EncDec A} : EncDec (option A).
-Proof.
-  split.
-  - intros v. unfold decode, encode.
-    destruct v; simpl. rewrite encdec. eauto. eauto.
-  - intros v w Heq.
-    destruct w.
-    + unfold decode, encode in *.
-      unfold option_encodable, option_decodable in *.
-      destruct v; inversion Heq.
-      destruct v; inversion Heq.
-      destruct l; inversion Heq.
-      f_equiv.
-      apply decenc.
-        by destruct (decode v); inversion Heq.
-    + unfold decode, encode in *.
-      simpl.
-      unfold option_encodable, option_decodable in *.
-      destruct v; inversion Heq.
-      * destruct v; inversion Heq.
-        destruct l; inversion Heq.
-        eauto.
-      * destruct (decode v); inversion Heq.
-Qed.
-
-Lemma enc_dec {A : Type} `{ED : EncDec A}
-      v (w : A) : encode w = v <-> decode v = Some w.
-Proof.
-  split.
-  - intros.
-    rewrite -encdec.
-    rewrite -H.
-    reflexivity.
-  - intros.
-    apply decenc. eauto.
-Qed.
-
-Lemma enc_inj {A : Type} `{ED : EncDec A}
-      x y : encode x = encode y -> x = y.
-Proof.
-  intros Heq.
-  assert (decode (encode x) = decode (encode y)).
-  { by f_equiv. }
-  erewrite encdec in H=> //.
-  erewrite encdec in H=> //.
-  by inversion H.
+  - intros []=> //. by rewrite /= val_encode_decode.
+  - intros [] ??; repeat (simplify_option_eq || case_match);
+      by repeat match goal with
+      | H : val_decode _ = Some _ |- _ => apply val_decode_encode in H as <-
+      end.
 Qed.
