theories/examples/branching_proofs.v
@@ -1,13 +1,16 @@
-From iris.proofmode Require Import tactics.
-From iris.program_logic Require Export weakestpre.
 From iris.heap_lang Require Import proofmode notation.
-From iris.base_logic Require Import invariants.
 From osiris.proto Require Import branching.
-From osiris.examples Require Import branching_examples.
+
+Definition branch_example b : expr :=
+  (let: "c" := new_chan #() in
+   select "c" #Left #b;;
+   Fork(branch: "c" @ #Right
+    left  send "c" #Right #5
+    right #());;
+   (if: #b then recv "c" #Left else #()))%E.
 
 Section BranchingExampleProofs.
-  Context `{!heapG Σ} (N : namespace).
-  Context `{!logrelG val Σ}.
+  Context `{!heapG Σ, !logrelG val Σ}.
 
   Lemma branch_proof b :
     {{{ True }}}
@@ -17,29 +20,24 @@ Section BranchingExampleProofs.
                   | Right => ⌜v = #()⌝
                   end }}}.
   Proof.
-    iIntros (Φ H) "HΦ".
+    iIntros (Φ _) "HΦ".
     rewrite /branch_example.
-    wp_apply (new_chan_st_spec N
-      ((<?> v @ ⌜v = 5⌝, TEnd) <+> (TEnd)))=> //;
+    wp_apply (new_chan_st_spec nroot ((<?> v @ ⌜v = 5⌝, TEnd) <+> TEnd))=> //;
     iIntros (c γ) "[Hstl Hstr]".
-    wp_apply (select_st_spec with "Hstl");
-    iIntros "Hstl".
+    wp_apply (select_st_spec with "Hstl"); iIntros "Hstl".
     wp_pures.
     wp_apply (wp_fork with "[Hstr]").
     - iNext.
       simpl.
       wp_apply (branch_st_spec with "Hstr")=> //;
-      iIntros (v) "[Hstr | Hstr]"; iDestruct "Hstr" as (->) "Hstr".
-      + wp_pures. 
-        wp_apply (send_st_spec N Z with "[$Hstr //]").
-        iIntros "Hstr". done.
-      + wp_pures. done.
+      iIntros (v) "[[-> Hstr]|[-> Hstr]]".
+      + wp_pures.
+        wp_apply (send_st_spec (A:=Z) with "[$Hstr //]"); auto.
+      + by wp_pures.
     - destruct b.
-      + wp_apply (recv_st_spec N Z with "Hstl");
-        iIntros (v) "[Hstl HP]".
-        iDestruct "HP" as %->.
+      + wp_apply (recv_st_spec (A:=Z) with "Hstl");
+        iIntros (v) "[Hstl ->]".
         by iApply "HΦ".
       + wp_pures. by iApply "HΦ".
   Qed.
-
 End BranchingExampleProofs.
