theories/examples/proofs_enc.v
@@ -1,28 +1,65 @@
-From iris.proofmode Require Import tactics.
-From iris.program_logic Require Export weakestpre.
 From iris.heap_lang Require Import proofmode notation.
-From iris.algebra Require Import list auth excl.
-From iris.base_logic Require Import invariants.
 From osiris.proto Require Import proto_enc.
-From osiris.examples Require Import examples.
+
+Definition seq_example : expr :=
+  (let: "c" := new_chan #() in
+   send "c" #Left #5;;
+   recv "c" #Right)%E.
+
+Definition par_example : expr :=
+  (let: "c" := new_chan #() in
+   Fork(send "c" #Left #5);;
+   recv "c" #Right)%E.
+
+Definition par_2_example : expr :=
+  (let: "c" := new_chan #() in
+   Fork(let: "v" := recv "c" #Right in send "c" #Right ("v"+#2));;
+   send "c" #Left #5;;recv "c" #Left)%E.
+
+Definition heaplet_example : expr :=
+  (let: "c" := new_chan #() in
+   Fork(send "c" #Left (ref #5));;
+   !(recv "c" #Right))%E.
+
+Definition channel_example : expr :=
+  (let: "c" := new_chan #() in
+   Fork(
+       let: "c'" := new_chan #() in
+       send "c" #Left ("c'");; send "c'" #Left #5);;
+   let: "c'" := recv "c" #Right in
+   recv "c'" #Right
+  )%E.
+
+Definition bad_seq_example : expr :=
+  (let: "c" := new_chan #() in
+   let: "v" := recv "c" #Right in
+   send "c" #Left #5;; "v")%E.
+
+Definition bad_par_example : expr :=
+  (let: "c" := new_chan #() in
+   Fork(#());;
+   recv "c" #Right)%E.
+
+Definition bad_interleave_example : expr :=
+  (let: "c" := new_chan #() in
+   let: "c'" := new_chan #() in
+   Fork(recv "c" #Right;; send "c'" #Right #5);;
+   recv "c'" #Left;; send "c" #Left #5)%E.
 
 Section ExampleProofsEnc.
-  Context `{!heapG Σ} (N : namespace).
-  Context `{!logrelG val Σ}.
+  Context `{!heapG Σ, !logrelG val Σ}.
 
   Lemma seq_proof :
     {{{ True }}} seq_example {{{ v, RET v; ⌜v = #5⌝ }}}.
   Proof.
-    iIntros (Φ H) "HΦ".
+    iIntros (Φ _) "HΦ".
     rewrite /seq_example.
-    wp_apply (new_chan_st_spec N (<!> v @ ⌜v = 5⌝, TEnd))=> //;
-    iIntros (c γ) "[Hstl Hstr]"=> /=.
-    wp_apply (send_st_spec N Z with "[$Hstl //]");
-    iIntros "Hstl".
-    wp_apply (recv_st_spec N Z with "[Hstr]"). iApply "Hstr".
-    iIntros (v) "[Hstr HP]".
+    wp_apply (new_chan_st_spec nroot (<!> v @ ⌜v = 5⌝, TEnd))=> //;
+      iIntros (c γ) "[Hstl Hstr]"=> /=.
+    wp_apply (send_st_spec (A:=Z) with "[$Hstl //]"); iIntros "Hstl".
+    wp_apply (recv_st_spec (A:=Z) with "Hstr").
+    iIntros (v) "[Hstr ->]".
     iApply "HΦ".
-    iDestruct "HP" as %->.
     eauto.
   Qed.
 
@@ -31,44 +68,34 @@ Section ExampleProofsEnc.
       par_2_example
     {{{ (v:Z), RET #v; ⌜7 ≤ v⌝ }}}.
   Proof.
-    iIntros (Φ H) "HΦ".
+    iIntros (Φ _) "HΦ".
     rewrite /par_2_example.
-    wp_apply (new_chan_st_spec N
-      (<!> v @ ⌜5 ≤ v⌝,
-               <?> v' @ ⌜v+2 ≤ v'⌝,
-                        TEnd))=> //;
+    wp_apply (new_chan_st_spec nroot
+      (<!> v @ ⌜5 ≤ v⌝, <?> v' @ ⌜v+2 ≤ v'⌝, TEnd))=> //;
     iIntros (c γ) "[Hstl Hstr]"=> /=.
     wp_apply (wp_fork with "[Hstr]").
     - iNext.
-      wp_apply (recv_st_spec N Z with "Hstr");
-      iIntros (v) "[Hstr HP]".
-      wp_apply (send_st_spec N Z with "[$Hstr //]");
-      iIntros "Hstr".
+      wp_apply (recv_st_spec (A:=Z) with "Hstr"); iIntros (v) "[Hstr HP]".
+      wp_apply (send_st_spec (A:=Z) with "[$Hstr //]"); iIntros "Hstr".
       eauto.
-    - wp_apply (send_st_spec N Z with "[$Hstl //]");
-      iIntros "Hstl".
-      wp_apply (recv_st_spec N Z with "Hstl");
-      iIntros (v) "[Hstl HP]".
-      iApply "HΦ".
-      iDestruct "HP" as %HP.
-      iPureIntro. lia.
+    - wp_apply (send_st_spec (A:=Z) with "[$Hstl //]"); iIntros "Hstl".
+      wp_apply (recv_st_spec (A:=Z) with "Hstl"); iIntros (v) "[Hstl %]".
+      iApply "HΦ". iPureIntro. lia.
   Qed.
 
   Lemma heaplet_proof :
     {{{ True }}} heaplet_example {{{ v l, RET v; ⌜v = #5⌝ ∗ l ↦ v }}}.
   Proof.
     rewrite /heaplet_example.
-    iIntros (Φ H) "HΦ".
-    wp_apply (new_chan_st_spec N (<!> v @ (v ↦ #5), TEnd))=> //;
+    iIntros (Φ _) "HΦ".
+    wp_apply (new_chan_st_spec nroot (<!> v @ (v ↦ #5), TEnd))=> //;
     iIntros (c γ) "[Hstl Hstr]"=> /=.
     wp_apply (wp_fork with "[Hstl]").
     - iNext.
       wp_alloc l as "HP".
-      wp_apply (send_st_spec N loc with "[$Hstl HP]")=> //;
-      iIntros "Hstl".
+      wp_apply (send_st_spec (A:=loc) with "[$Hstl HP]")=> //; iIntros "Hstl".
       eauto.
-    - wp_apply (recv_st_spec N loc with "Hstr");
-      iIntros (v) "[Hstr HP]".
+    - wp_apply (recv_st_spec (A:=loc) with "Hstr"); iIntros (v) "[Hstr HP]".
       wp_load.
       iApply "HΦ".
       by iFrame.
@@ -77,43 +104,36 @@ Section ExampleProofsEnc.
   Lemma channel_proof :
     {{{ True }}} channel_example {{{ v, RET v; ⌜v = #5⌝ }}}.
   Proof.
-    iIntros (Φ H) "HΦ".
+    iIntros (Φ _) "HΦ".
     rewrite /channel_example.
-    wp_apply (new_chan_st_spec N
-      (<!> v @ (∃ γ, ⟦ v @ Right : <?> v @ ⌜v = 5⌝, TEnd ⟧{N,γ}),
+    wp_apply (new_chan_st_spec nroot
+      (<!> v @ (∃ γ, ⟦ v @ Right : <?> v @ ⌜v = 5⌝, TEnd ⟧{nroot,γ}),
                TEnd))=> //;
     iIntros (c γ) "[Hstl Hstr]"=> /=.
     wp_apply (wp_fork with "[Hstl]").
     - iNext.
-      wp_apply (new_chan_st_spec N (<!> v @ ⌜v = 5⌝, TEnd))=> //;
-      iIntros (c' γ') "[Hstl' Hstr']"=> /=.
-      wp_apply (send_st_spec N val with "[Hstl Hstr']");
+      wp_apply (new_chan_st_spec nroot (<!> v @ ⌜v = 5⌝, TEnd))=> //;
+        iIntros (c' γ') "[Hstl' Hstr']"=> /=.
+      wp_apply (send_st_spec (A:=val) with "[Hstl Hstr']");
         first by eauto 10 with iFrame.
       iIntros "Hstl".
-      wp_apply (send_st_spec N Z with "[$Hstl' //]");
-      iIntros "Hstl'".
+      wp_apply (send_st_spec (A:=Z) with "[$Hstl' //]"); iIntros "Hstl'".
       eauto.
-    - wp_apply (recv_st_spec N val with "Hstr");
-      iIntros (v) "[Hstr Hstr']".
+    - wp_apply (recv_st_spec (A:=val) with "Hstr"); iIntros (v) "[Hstr Hstr']".
       iDestruct "Hstr'" as (γ') "Hstr'".
-      wp_apply (recv_st_spec N Z with "Hstr'");
-      iIntros (v') "[Hstr' HP]".
-      iDestruct "HP" as %<-.
+      wp_apply (recv_st_spec (A:=Z) with "Hstr'"); iIntros (v') "[Hstr' <-]".
       by iApply "HΦ".
   Qed.
 
   Lemma bad_seq_proof :
     {{{ True }}} bad_seq_example {{{ v, RET v; ⌜v = #5⌝ }}}.
   Proof.
-    iIntros (Φ H) "HΦ".
+    iIntros (Φ _) "HΦ".
     rewrite /bad_seq_example.
-    wp_apply (new_chan_st_spec N (<!> v @ ⌜v = 5⌝, TEnd))=> //;
+    wp_apply (new_chan_st_spec nroot (<!> v @ ⌜v = 5⌝, TEnd))=> //;
     iIntros (c γ) "[Hstl Hstr]"=> /=.
-    wp_apply (recv_st_spec N Z with "Hstr");
-    iIntros (v) "[Hstr HP]".
-    wp_apply (send_st_spec N Z with "[$Hstl //]");
-    iIntros "Hstl".
-    iDestruct "HP" as %->.
+    wp_apply (recv_st_spec (A:=Z) with "Hstr"); iIntros (v) "[Hstr ->]".
+    wp_apply (send_st_spec (A:=Z) with "[$Hstl //]"); iIntros "Hstl".
     wp_pures.
     by iApply "HΦ".
   Qed.
@@ -121,36 +141,30 @@ Section ExampleProofsEnc.
   Lemma bad_par_proof :
     {{{ True }}} bad_par_example {{{ v, RET v; ⌜v = #5⌝ }}}.
   Proof.
-    iIntros (Φ H) "HΦ".
+    iIntros (Φ _) "HΦ".
     rewrite /bad_par_example.
-    wp_apply (new_chan_st_spec N (<!> v @ ⌜v = 5⌝, TEnd))=> //;
+    wp_apply (new_chan_st_spec nroot (<!> v @ ⌜v = 5⌝, TEnd))=> //;
     iIntros (c γ) "[Hstl Hstr]"=> /=.
     wp_apply (wp_fork with "[Hstl]").
     - iNext. by wp_finish.
-    - wp_apply (recv_st_spec _ with "Hstr");
-      iIntros (v) "[Hstr HP]".
-      iDestruct "HP" as %->.
+    - wp_apply (recv_st_spec (A:=Z) with "Hstr"); iIntros (v) "[Hstr ->]".
       by iApply "HΦ".
   Qed.
 
   Lemma bad_interleave_proof :
     {{{ True }}} bad_interleave_example {{{ v, RET v; ⌜v = #()⌝ }}}.
   Proof.
-    iIntros (Φ H) "HΦ".
+    iIntros (Φ _) "HΦ".
     rewrite /bad_interleave_example.
-    wp_apply (new_chan_st_spec N (<!> v @ ⌜v = 5⌝, TEnd))=> //;
+    wp_apply (new_chan_st_spec nroot (<!> v @ ⌜v = 5⌝, TEnd))=> //;
     iIntros (c γ) "[Hstl Hstr]"=> /=.
-    wp_apply (new_chan_st_spec N (<?> v @ ⌜v = 5⌝, TEnd))=> //;
+    wp_apply (new_chan_st_spec nroot (<?> v @ ⌜v = 5⌝, TEnd))=> //;
     iIntros (c' γ') "[Hstl' Hstr']"=> /=.
     wp_apply (wp_fork with "[Hstr Hstr']").
-    - iNext. wp_apply (recv_st_spec _ with "Hstr");
-      iIntros (v) "[Hstr HP]".
-      wp_apply (send_st_spec _ Z with "[$Hstr' //]"). eauto.
-    - wp_apply (recv_st_spec _ Z with "[$Hstl' //]");
-      iIntros (v) "[Hstl' HP]".
-      wp_apply (send_st_spec _ Z with "[$Hstl //]");
-      iIntros "Hstl".
+    - iNext. wp_apply (recv_st_spec (A:=Z) with "Hstr"); iIntros (v) "[Hstr HP]".
+      wp_apply (send_st_spec (A:=Z) with "[$Hstr' //]"). eauto.
+    - wp_apply (recv_st_spec (A:=Z) with "[$Hstl' //]"); iIntros (v) "[Hstl' HP]".
+      wp_apply (send_st_spec (A:=Z) with "[$Hstl //]"); iIntros "Hstl".
       by iApply "HΦ".
   Qed.
-
 End ExampleProofsEnc.
