theories/proto/proto_enc.v
@@ -1,18 +1,14 @@
-From iris.proofmode Require Import tactics.
-From iris.program_logic Require Export weakestpre.
 From iris.heap_lang Require Import proofmode notation.
-From iris.algebra Require Import list auth excl.
-From iris.base_logic Require Import invariants.
 From osiris.proto Require Export encodable proto_specs.
 
 Section DualProtoEnc.
-  Context `{EncDec V} `{PROP: bi} .
+  Context `{ValEncDec V} {PROP: bi} .
 
   Definition TSR'
-    (a : action) (P : V → PROP) (prot : V → proto val PROP) : proto val PROP :=
-  TSR a
-    (λ v, if decode v is Some x then P x else False)%I
-    (λ v, if decode v is Some x then prot x else TEnd (* dummy *)).
+      (a : action) (P : V → PROP) (prot : V → proto val PROP) : proto val PROP :=
+    TSR a
+      (λ v, if val_decode v is Some x then P x else False)%I
+      (λ v, if val_decode v is Some x then prot x else TEnd (* dummy *)).
   Global Instance: Params (@TSR') 3.
 
   Global Instance is_dual_tsr' a1 a2 P (st1 st2 : V → proto val PROP) :
@@ -22,10 +18,9 @@ Section DualProtoEnc.
   Proof.
     rewrite /IsDualAction /IsDualProto. intros <- Hst.
     rewrite -(proto_force_eq (dual_proto _)).
-    constructor=> x. done. destruct (decode x)=> //.
+    constructor=> x. done. destruct (val_decode x)=> //.
     apply is_dual_end.
   Qed.
-
 End DualProtoEnc.
 
 Notation "<!> x @ P , prot" :=
@@ -44,46 +39,35 @@ Notation "<?> @ P , prot" := (<?> dummy__ @ P dummy__, prot dummy__)%proto
   (at level 200, prot at level 200) : proto_scope.
 
 Section proto_enc_specs.
-  Context `{!heapG Σ} (N : namespace).
-  Context `{!logrelG val Σ}.
+  Context `{!heapG Σ, !logrelG val Σ} `{ValEncDec A} (N : namespace).
 
-  Lemma send_st_spec (A : Type) `{EncDec A}
-        prot γ c s (P : A → iProp Σ) w :
+  Lemma send_st_spec prot γ c s (P : A → iProp Σ) w :
     {{{ P w ∗ ⟦ c @ s : <!> @ P, prot ⟧{N,γ} }}}
-      send c #s (encode w)
+      send c #s (val_encode w)
     {{{ RET #(); ⟦ c @ s : prot w ⟧{N,γ} }}}.
   Proof.
     iIntros (Φ) "[HP Hsend] HΦ".
-    iApply (send_st_spec with "[HP Hsend]").
-    simpl.
-    iFrame.
-    by rewrite encdec.
-    iNext.
-    rewrite encdec.
+    iApply (send_st_spec with "[HP $Hsend]").
+    { by rewrite val_encode_decode. }
+    iNext. rewrite val_encode_decode.
     by iApply "HΦ".
   Qed.
 
-  Lemma recv_st_spec (A : Type) `{EncDec A}
-        prot γ c s (P : A → iProp Σ) :
+  Lemma recv_st_spec prot γ c s (P : A → iProp Σ) :
     {{{ ⟦ c @ s : <?> @ P, prot ⟧{N,γ} }}}
       recv c #s
-    {{{ v, RET (encode v); ⟦ c @ s : prot v ⟧{N,γ} ∗ P v }}}.
+    {{{ v, RET (val_encode v); ⟦ c @ s : prot v ⟧{N,γ} ∗ P v }}}.
   Proof.
     iIntros (Φ) "Hrecv HΦ".
     iApply (recv_st_spec with "Hrecv").
     iNext. iIntros (v).
     iIntros "[H HP]".
-    iAssert ((∃ w, ⌜decode v = Some w⌝ ∗ P w)%I) with "[HP]" as (w Hw) "HP".
-    { destruct (decode v).
-      iExists a. by iFrame. iDestruct "HP" as %HP=>//. }
+    iAssert (∃ w, ⌜val_decode v = Some w⌝ ∗ P w)%I with "[HP]" as (w Hw) "HP".
+    { destruct (val_decode v) as [x|]; last done.
+      iExists x. by iFrame. }
     iSpecialize ("HΦ" $!w).
-    apply enc_dec in Hw. rewrite Hw.
-    iApply "HΦ".
-    iFrame.
-    apply enc_dec in Hw.
-    destruct (decode v).
-    - inversion Hw. subst. iApply "H".
-    - inversion Hw.
+    apply val_decode_encode in Hw as <-.
+    iApply "HΦ". iFrame "HP".
+    by rewrite val_encode_decode.
   Qed.
-
 End proto_enc_specs.
